ContextBasicDenotation/theories/TermOpen.v
@@ -5,22 +5,24 @@
 From ContextBasicDenotation Require Import Notation StoreTyping.
 From ContextBasicDenotation Require Import TermSyntax TermEval.
 From ContextBase Require Import BaseTactics.
+From ContextQualifier Require Import Qualifier.
 
 Section TermDenotation.
 
-Definition expr_result_lqual (e : tm) (x : logic_var) : logic_qualifier :=
-  lqual (tm_lvars e ∪ {[x]})
-    (fun w => expr_result_at_world e x (@lw value _ w : LWorldT)).
+Definition expr_result_qual (e : tm) (x : logic_var) : qualifier (V := value) :=
+  tqual (tm_lvars e ∪ {[x]})
+    (fun s => expr_result_at_store e x (lso_store s)).
 
 Definition expr_result_formula (e : tm) (x : logic_var) : Formula :=
-  FAtom (expr_result_lqual e x).
+  FFiberAtom (expr_result_qual e x).
 
 Lemma formula_fv_expr_result_formula e x :
   formula_fv (expr_result_formula e x) =
   lvars_fv (tm_lvars e ∪ {[x]}).
 Proof.
-  unfold expr_result_formula, expr_result_lqual.
-  rewrite formula_fv_atom. reflexivity.
+  unfold expr_result_formula, expr_result_qual.
+  rewrite formula_fv_fiber_atom.
+  reflexivity.
 Qed.
 
 Lemma lstore_swap_lookup_inv_value a b (σ : LStoreT) z :
@@ -282,15 +284,29 @@ Lemma formula_open_expr_total_formula k y e :
   expr_total_formula (open_tm k (vfvar y) e).
 Proof.
   intros Hy.
-  unfold expr_total_formula, expr_total_lqual.
-  cbn [formula_open lqual_open].
-  f_equal.
-  apply logic_qualifier_ext.
+  unfold expr_total_formula, expr_total_qual.
+  rewrite formula_open_fiber_atom.
+  apply f_equal.
+  apply qual_ext.
   - symmetry. apply tm_lvars_open. exact Hy.
-  - intros w1 w2 Hlw. cbn [lqual_prop].
-    transitivity (expr_total_on (open_tm k (vfvar y) e) (@lw value _ w1)).
-    + apply expr_total_on_open_back_iff. exact Hy.
-    + rewrite Hlw. reflexivity.
+  - intros s1 s2 Hs. cbn [qual_prop qual_lvars].
+    split; intros [v Heval]; exists v.
+    + apply expr_eval_in_store_open_back_iff in Heval.
+      * change (expr_eval_in_store (lso_store s2)
+          (open_tm k (vfvar y) e) v).
+        rewrite <- Hs. exact Heval.
+      * exact Hy.
+      * change (lvars_open k y (tm_lvars e) ⊆
+          dom (lso_store s1 : LStoreT)).
+        rewrite (lso_dom s1). reflexivity.
+    + apply expr_eval_in_store_open_back_iff.
+      * exact Hy.
+      * change (lvars_open k y (tm_lvars e) ⊆
+          dom (lso_store s1 : LStoreT)).
+        rewrite (lso_dom s1). reflexivity.
+      * change (expr_eval_in_store (lso_store s1)
+          (open_tm k (vfvar y) e) v).
+        rewrite Hs. exact Heval.
 Qed.
 
 Lemma expr_result_at_store_open_back_iff k y e z σ :
@@ -403,17 +419,31 @@ Lemma formula_open_expr_result_formula k y e z :
     (open_tm k (vfvar y) e) (logic_var_open k y z).
 Proof.
   intros Hy.
-  unfold expr_result_formula, expr_result_lqual.
-  cbn [formula_open lqual_open].
-  f_equal.
-  apply logic_qualifier_ext.
+  unfold expr_result_formula, expr_result_qual.
+  rewrite formula_open_fiber_atom.
+  apply f_equal.
+  apply qual_ext.
   - apply tm_lvars_open_result_domain. exact Hy.
-  - intros w1 w2 Hlw. cbn [lqual_prop].
-    transitivity (expr_result_at_world
-      (open_tm k (vfvar y) e) (logic_var_open k y z)
-      (@lw value _ w1)).
-    + apply expr_result_at_world_open_back_iff. exact Hy.
-    + rewrite Hlw. reflexivity.
+  - intros s1 s2 Hs. cbn [qual_prop qual_lvars].
+    split; intros Hres.
+    + apply expr_result_at_store_open_back_iff in Hres.
+      * change (expr_result_at_store
+          (open_tm k (vfvar y) e) (logic_var_open k y z)
+          (lso_store s2)).
+        rewrite <- Hs. exact Hres.
+      * exact Hy.
+      * change (lvars_open k y (tm_lvars e) ⊆
+          dom (lso_store s1 : LStoreT)).
+        rewrite (lso_dom s1). set_solver.
+    + apply expr_result_at_store_open_back_iff.
+      * exact Hy.
+      * change (lvars_open k y (tm_lvars e) ⊆
+          dom (lso_store s1 : LStoreT)).
+        rewrite (lso_dom s1). set_solver.
+      * change (expr_result_at_store
+          (open_tm k (vfvar y) e) (logic_var_open k y z)
+          (lso_store s1)).
+        rewrite Hs. exact Hres.
 Qed.
 
 Lemma formula_open_env_expr_total_formula η e :
