ContextQualifier/theories/Qualifier.v
@@ -1,0 +1,635 @@
+(** * ContextQualifier.Qualifier
+
+    Store-level qualifiers are locally-nameless predicates over lvar-keyed
+    stores.  This mirrors [LogicQualifier]'s dependent-domain design, except
+    the payload is an [LStore] rather than an [LWorld].
+
+    The core language operation is opening.  Opening is implemented as a swap
+    between a bound lvar and a free atom, with the predicate interpreting its
+    input after swapping the store back. *)
+
+From CoreLang Require Export Prelude Syntax.
+From ContextBase Require Export Prelude LogicVar LogicVarShift LogicVarOpenEnv
+  BaseTactics.
+From ContextStore Require Export Store.
+From Stdlib Require Import Logic.FunctionalExtensionality
+  Logic.ProofIrrelevance Logic.PropExtensionality.
+
+Section Qualifier.
+
+Context {V : Type} `{ValueSig V}.
+
+Local Notation LStoreT := (LStore (V := V)) (only parsing).
+Local Notation LStoreOnT := (LStoreOn (V := V)) (only parsing).
+Local Notation StoreT := (Store (V := V)) (only parsing).
+
+Record qualifier : Type := tqual {
+  qual_lvars : lvset;
+  qual_prop : LStoreOnT qual_lvars -> Prop;
+}.
+
+Definition qual_vars (q : qualifier) : lvset :=
+  qual_lvars q.
+
+Definition qual_dom (q : qualifier) : aset :=
+  lvars_fv (qual_lvars q).
+
+Definition qual_bvars (q : qualifier) : gset nat :=
+  lvars_bv (qual_lvars q).
+
+Lemma qual_ext (q1 q2 : qualifier) :
+  qual_lvars q1 = qual_lvars q2 ->
+  (forall (s1 : LStoreOnT (qual_lvars q1))
+          (s2 : LStoreOnT (qual_lvars q2)),
+      lso_store s1 = lso_store s2 ->
+      qual_prop q1 s1 <-> qual_prop q2 s2) ->
+  q1 = q2.
+Proof.
+  destruct q1 as [D1 P1], q2 as [D2 P2]. simpl.
+  intros HD HP. subst D2. f_equal.
+  apply functional_extensionality. intros s.
+  apply propositional_extensionality.
+  apply HP. reflexivity.
+Qed.
+
+Definition qual_open_atom
+    (k : nat) (x : atom) (q : qualifier) : qualifier :=
+  match q with
+  | tqual D P =>
+      tqual (lvars_open k x D)
+        (fun s => P (lstore_on_open_back k x D s))
+  end.
+
+Definition lstore_on_atom_swap_back
+    (x y : atom) (D : lvset)
+    (s : LStoreOnT (lvars_swap x y D)) : LStoreOnT D.
+Proof.
+  refine {| storeAO_store := lstore_swap (LVFree x) (LVFree y) (lso_store s) |}.
+  unfold lstore_swap, lstore_rekey.
+  rewrite storeA_rekey_dom by apply swap_inj.
+  change (set_swap (LVFree x) (LVFree y) (dom (lso_store s : LStoreT)) = D).
+  rewrite (lso_dom s).
+  better_base_solver.
+Defined.
+
+Definition lstore_on_atom_swap_front
+    (x y : atom) (D : lvset)
+    (s : LStoreOnT D) : LStoreOnT (lvars_swap x y D).
+Proof.
+  refine {| storeAO_store := lstore_swap (LVFree x) (LVFree y) (lso_store s) |}.
+  unfold lstore_swap, lstore_rekey.
+  rewrite storeA_rekey_dom by apply swap_inj.
+  change (set_swap (LVFree x) (LVFree y) (dom (lso_store s : LStoreT)) =
+    lvars_swap x y D).
+  rewrite (lso_dom s). reflexivity.
+Defined.
+
+Lemma lstore_on_atom_swap_back_front x y D (s : LStoreOnT D) :
+  lstore_on_atom_swap_back x y D
+    (lstore_on_atom_swap_front x y D s) = s.
+Proof.
+  apply lstore_on_ext.
+  unfold lstore_on_atom_swap_back, lstore_on_atom_swap_front.
+  cbn [lso_store storeAO_store].
+  change (lstore_swap (LVFree x) (LVFree y)
+    (lstore_swap (LVFree x) (LVFree y) (lso_store s)) = lso_store s).
+  unfold lstore_swap, lstore_rekey.
+  apply storeA_swap_involutive.
+Qed.
+
+Lemma lstore_on_atom_swap_front_back x y D
+    (s : LStoreOnT (lvars_swap x y D)) :
+  lstore_on_atom_swap_front x y D
+    (lstore_on_atom_swap_back x y D s) = s.
+Proof.
+  apply lstore_on_ext.
+  unfold lstore_on_atom_swap_back, lstore_on_atom_swap_front.
+  cbn [lso_store storeAO_store].
+  change (lstore_swap (LVFree x) (LVFree y)
+    (lstore_swap (LVFree x) (LVFree y) (lso_store s)) = lso_store s).
+  unfold lstore_swap, lstore_rekey.
+  apply storeA_swap_involutive.
+Qed.
+
+Definition qual_atom_swap
+    (x y : atom) (q : qualifier) : qualifier :=
+  match q with
+  | tqual D P =>
+      tqual (lvars_swap x y D)
+        (fun s => P (lstore_on_atom_swap_back x y D s))
+  end.
+
+Lemma qual_atom_swap_involutive x y (q : qualifier) :
+  qual_atom_swap x y (qual_atom_swap x y q) = q.
+Proof.
+  destruct q as [D P]. cbn [qual_atom_swap].
+  apply qual_ext.
+  - apply set_swap_involutive.
+  - intros s1 s2 Hs. cbn [qual_prop qual_lvars].
+    enough (lstore_on_atom_swap_back x y D
+      (lstore_on_atom_swap_back x y (lvars_swap x y D) s1) = s2) as ->.
+    { reflexivity. }
+    apply lstore_on_ext.
+    unfold lstore_on_atom_swap_back. cbn [lso_store storeAO_store].
+    change (lstore_swap (LVFree x) (LVFree y)
+      (lstore_swap (LVFree x) (LVFree y) (lso_store s1)) = lso_store s2).
+    rewrite Hs.
+    unfold lstore_swap, lstore_rekey.
+    apply storeA_swap_involutive.
+Qed.
+
+Lemma qual_atom_swap_fresh_id x y (q : qualifier) :
+  x ∉ qual_dom q ->
+  y ∉ qual_dom q ->
+  qual_atom_swap x y q = q.
+Proof.
+  destruct q as [D P]. cbn [qual_atom_swap qual_dom qual_lvars].
+  intros Hx Hy.
+  apply qual_ext.
+  - apply lvars_swap_fresh; assumption.
+  - intros s1 s2 Hs. cbn [qual_prop qual_lvars].
+    enough (lstore_on_atom_swap_back x y D s1 = s2) as -> by reflexivity.
+    apply lstore_on_ext.
+    unfold lstore_on_atom_swap_back. cbn [lso_store storeAO_store].
+    change (lstore_swap (LVFree x) (LVFree y) (lso_store s1) =
+      lso_store s2).
+    rewrite Hs.
+    apply storeA_swap_fresh.
+    + intros Hbad. apply Hx. apply lvars_fv_elem.
+      rewrite <- (lso_dom s2). exact Hbad.
+    + intros Hbad. apply Hy. apply lvars_fv_elem.
+      rewrite <- (lso_dom s2). exact Hbad.
+Qed.
+
+Lemma qual_atom_swap_open_conjugate k x y z q :
+  qual_atom_swap x y (qual_open_atom k (swap x y z) q) =
+  qual_open_atom k z (qual_atom_swap x y q).
+Proof.
+  destruct q as [D P]. cbn [qual_atom_swap qual_open_atom].
+  apply qual_ext.
+  - apply lvars_swap_open_conjugate.
+  - intros s1 s2 Hs. cbn [qual_prop qual_lvars].
+    enough
+      (lstore_on_open_back k (swap x y z) D
+        (lstore_on_atom_swap_back x y (lvars_open k (swap x y z) D) s1) =
+       lstore_on_atom_swap_back x y D
+        (lstore_on_open_back k z (lvars_swap x y D) s2)) as ->.
+    { reflexivity. }
+    apply lstore_on_ext.
+    unfold lstore_on_open_back, lstore_on_atom_swap_back.
+    cbn [lso_store storeAO_store].
+    change (lstore_swap (LVBound k) (LVFree (swap x y z))
+      (lstore_swap (LVFree x) (LVFree y) (lso_store s1)) =
+      lstore_swap (LVFree x) (LVFree y)
+        (lstore_swap (LVBound k) (LVFree z) (lso_store s2))).
+    rewrite Hs.
+    unfold lstore_swap, lstore_rekey.
+    change (storeA_swap (LVBound k) (LVFree (swap x y z))
+      (storeA_swap (LVFree x) (LVFree y) (lso_store s2) : LStoreT) =
+      storeA_swap (LVFree x) (LVFree y)
+        (storeA_swap (LVBound k) (LVFree z) (lso_store s2) : LStoreT)).
+    rewrite (storeA_swap_conjugate_inv
+      (LVFree x) (LVFree y) (LVBound k) (LVFree (swap x y z))).
+    replace (swap (LVFree x) (LVFree y) (LVBound k)) with (LVBound k)
+      by (unfold swap; repeat destruct decide; congruence).
+    replace (swap (LVFree x) (LVFree y) (LVFree (swap x y z)))
+      with (LVFree z)
+      by (unfold swap; repeat destruct decide; congruence).
+    reflexivity.
+Qed.
+
+Definition qual_mlsubst (ρ : LStoreT) (q : qualifier) : qualifier :=
+  match q with
+  | tqual D P =>
+      tqual (D ∖ dom (ρ : gmap logic_var V))
+        (fun s => P (lstore_on_mlsubst_back D ρ s))
+  end.
+
+Lemma qual_mlsubst_empty (q : qualifier) :
+  qual_mlsubst (∅ : LStoreT) q = q.
+Proof.
+  destruct q as [D P]. cbn [qual_mlsubst].
+  apply qual_ext.
+  - change (D ∖ (∅ : lvset) = D).
+    apply difference_empty_L.
+  - intros s1 s2 Hs. cbn [qual_prop qual_lvars].
+    enough (lstore_on_mlsubst_back D (∅ : LStoreT) s1 = s2) as ->.
+    { reflexivity. }
+    apply lstore_on_ext.
+    unfold lstore_on_mlsubst_back. cbn [lso_store storeAO_store].
+    change ((@union (gmap logic_var V) _ (lso_store s1)
+      (storeA_restrict (∅ : LStoreT) D) : LStoreT) = lso_store s2).
+    rewrite Hs.
+    assert (Hempty : storeA_restrict (∅ : LStoreT) D = (∅ : LStoreT)).
+    {
+      apply storeA_map_eq. intros v.
+      rewrite storeA_restrict_lookup_none_l; [reflexivity|].
+      rewrite lookup_empty. reflexivity.
+    }
+    rewrite Hempty.
+    rewrite (right_id_L ∅ (∪)). reflexivity.
+Qed.
+
+Lemma qual_atom_swap_mlsubst x y (ρ : LStoreT) q :
+  qual_atom_swap x y (qual_mlsubst ρ q) =
+  qual_mlsubst (lvar_store_swap x y ρ) (qual_atom_swap x y q).
+Proof.
+  destruct q as [D P]. cbn [qual_atom_swap qual_mlsubst].
+  apply qual_ext.
+  - transitivity (set_swap (LVFree x) (LVFree y) D ∖
+      set_swap (LVFree x) (LVFree y) (dom (ρ : LStoreT))).
+    + apply set_swap_difference.
+    + apply (f_equal (fun R =>
+        set_swap (LVFree x) (LVFree y) D ∖ R)).
+      symmetry. apply lvar_store_swap_dom.
+  - intros s1 s2 Hs. cbn [qual_prop qual_lvars].
+    enough (lstore_on_mlsubst_back D ρ
+      (lstore_on_atom_swap_back x y (D ∖ dom (ρ : LStoreT)) s1) =
+      lstore_on_atom_swap_back x y D
+        (lstore_on_mlsubst_back (lvars_swap x y D)
+          (lvar_store_swap x y ρ) s2)) as <-.
+    { reflexivity. }
+    apply lstore_on_ext.
+    unfold lstore_on_mlsubst_back, lstore_on_atom_swap_back.
+    cbn [lso_store storeAO_store].
+    change ((@union (gmap logic_var V) _
+        (lstore_swap (LVFree x) (LVFree y) (lso_store s1))
+        (storeA_restrict ρ D) : LStoreT) =
+      lstore_swap (LVFree x) (LVFree y)
+        (@union (gmap logic_var V) _ (lso_store s2)
+          (storeA_restrict (lvar_store_swap x y ρ) (lvars_swap x y D)))).
+    rewrite Hs.
+    unfold lstore_swap, lstore_rekey, lvar_store_swap.
+    change ((@union (gmap logic_var V) _
+        (storeA_swap (LVFree x) (LVFree y) (lso_store s2))
+        (storeA_restrict ρ D) : LStoreT) =
+      storeA_swap (LVFree x) (LVFree y)
+        (@union (gmap logic_var V) _ (lso_store s2)
+          (storeA_restrict (storeA_swap (LVFree x) (LVFree y) ρ)
+            (lvars_swap x y D)))).
+    rewrite storeA_swap_union.
+    f_equal.
+    rewrite storeA_restrict_swap.
+    rewrite storeA_swap_involutive.
+    reflexivity.
+Qed.
+
+Definition qual_msubst_store (σ : StoreT) (q : qualifier) :
+    qualifier :=
+  qual_mlsubst (atom_store_to_lvar_store σ) q.
+
+Definition qual_open_env (η : gmap nat atom) (q : qualifier) : qualifier :=
+  map_fold (fun k x acc => qual_open_atom k x acc) q η.
+
+Lemma qual_open_env_empty q :
+  qual_open_env ∅ q = q.
+Proof.
+  unfold qual_open_env. rewrite map_fold_empty. reflexivity.
+Qed.
+
+Definition qual_top : qualifier :=
+  tqual ∅ (fun _ => True).
+
+Definition qual_and (q1 q2 : qualifier) : qualifier :=
+  match q1, q2 with
+  | tqual D1 P1, tqual D2 P2 =>
+      tqual (D1 ∪ D2)
+        (fun s =>
+           P1 (lstore_on_restrict D1 s ltac:(set_solver)) /\
+           P2 (lstore_on_restrict D2 s ltac:(set_solver)))
+  end.
+
+Definition lc_qualifier (q : qualifier) : Prop :=
+  lc_lvars (qual_lvars q).
+
+Definition body_qualifier (q : qualifier) : Prop :=
+  exists L : aset, forall x : atom, x ∉ L -> lc_qualifier (qual_open_atom 0 x q).
+
+#[global] Instance stale_qualifier : Stale qualifier := qual_dom.
+Arguments stale_qualifier /.
+
+#[global] Instance open_qual_atom_inst : Open atom qualifier := qual_open_atom.
+Arguments open_qual_atom_inst /.
+
+#[global] Instance lc_qual_inst : Lc qualifier := lc_qualifier.
+Arguments lc_qual_inst /.
+
+Notation "q '^q^' x" := (qual_open_atom 0 x q) (at level 20).
+
+Lemma qual_open_atom_vars k x q :
+  qual_vars (qual_open_atom k x q) = lvars_open k x (qual_vars q).
+Proof.
+  destruct q. reflexivity.
+Qed.
+
+Lemma qual_open_env_vars η q :
+  open_env_fresh_for_lvars η (qual_vars q) ->
+  qual_vars (qual_open_env η q) = lvars_open_env η (qual_vars q).
+Proof.
+  revert q.
+  induction η as [|k x η Hnone Hfold IH] using fin_maps.map_fold_ind.
+  - intros q _. rewrite qual_open_env_empty, lvars_open_env_empty.
+    reflexivity.
+  - intros q Hfresh.
+    pose proof (IH q
+      ltac:(eapply open_env_fresh_for_lvars_insert_tail; eassumption))
+      as HIH.
+    change (qual_vars
+      (map_fold (fun k x acc => qual_open_atom k x acc) q (<[k:=x]> η)) =
+      lvars_open_env (<[k:=x]> η) (qual_vars q)).
+    rewrite (Hfold qualifier (fun k x acc => qual_open_atom k x acc)).
+    fold (qual_open_env η q).
+    rewrite qual_open_atom_vars.
+    rewrite HIH.
+    rewrite lvars_open_env_insert_fresh.
+    + reflexivity.
+    + exact Hnone.
+    + eapply open_env_fresh_for_lvars_insert_head; eassumption.
+Qed.
+
+Lemma qual_open_atom_dom_subset k x q :
+  qual_dom (qual_open_atom k x q) ⊆ qual_dom q ∪ {[x]}.
+Proof.
+  destruct q as [D P]. cbn [qual_dom qual_open_atom qual_lvars].
+  apply lvars_fv_open_subset.
+Qed.
+
+Lemma qual_open_commute_fvar i j x y q :
+  i <> j ->
+  x <> y ->
+  qual_open_atom i x (qual_open_atom j y q) =
+  qual_open_atom j y (qual_open_atom i x q).
+Proof.
+  intros Hij Hxy.
+  destruct q as [D P].
+  apply qual_ext.
+  - cbn [qual_lvars qual_open_atom].
+    rewrite set_swap_conjugate.
+    replace (swap (LVBound i) (LVFree x) (LVBound j))
+      with (LVBound j).
+    2:{ better_base_solver. }
+    replace (swap (LVBound i) (LVFree x) (LVFree y))
+      with (LVFree y).
+    2:{ better_base_solver. }
+    reflexivity.
+  - intros s1 s2 Hs.
+    cbn [qual_prop qual_open_atom].
+    assert (Hback :
+      lstore_on_open_back j y D
+        (lstore_on_open_back i x (lvars_open j y D) s1) =
+      lstore_on_open_back i x D
+        (lstore_on_open_back j y (lvars_open i x D) s2)).
+    {
+      apply lstore_on_ext.
+      cbn [lso_store].
+      unfold lstore_on_open_back. cbn [lso_store].
+      change (lstore_swap (LVBound j) (LVFree y)
+          (lstore_swap (LVBound i) (LVFree x) (lso_store s1)) =
+        lstore_swap (LVBound i) (LVFree x)
+          (lstore_swap (LVBound j) (LVFree y) (lso_store s2))).
+      rewrite <- Hs.
+      symmetry.
+      unfold lstore_swap, lstore_rekey.
+      apply storeA_swap_commute_fresh; congruence.
+    }
+    rewrite Hback. tauto.
+Qed.
+
+Lemma qual_open_atom_commute_fresh i j x y q :
+  i <> j ->
+  x <> y ->
+  qual_open_atom i x (qual_open_atom j y q) =
+  qual_open_atom j y (qual_open_atom i x q).
+Proof. apply qual_open_commute_fvar. Qed.
+
+Lemma qual_open_env_insert_fresh η k x q :
+  η !! k = None ->
+  open_env_avoids_atom x η ->
+  open_env_values_inj η ->
+  qual_open_env (<[k := x]> η) q =
+  qual_open_atom k x (qual_open_env η q).
+Proof.
+  intros Hfresh Havoid Hinj.
+  unfold qual_open_env.
+  apply (map_fold_insert_L (M:=gmap nat) (A:=atom) (B:=qualifier)
+    (fun k x acc => qual_open_atom k x acc) q k x η).
+  - intros i j xi xj acc Hij Hi Hj.
+    apply qual_open_commute_fvar; [exact Hij|].
+    intros Heq. subst xj.
+    pose proof (open_env_values_inj_insert k x η Hfresh Havoid Hinj)
+      as Hinj'.
+    apply Hij. eapply Hinj'; eassumption.
+  - exact Hfresh.
+Qed.
+
+(** ** Qualifier Renaming
+
+    Opening remains the primitive operation in [Qualifier.v], because it is the
+    same involutive swap used by logic qualifiers.  Context-type denotation also needs
+    binder-depth shifts; those are represented here as a renaming transport:
+    the domain is renamed, and the new predicate holds exactly when the input
+    store is the renamed image of an old input store satisfying the old
+    predicate. *)
+
+Definition qual_rename
+    (f : logic_var -> logic_var) (Hf : Inj (=) (=) f)
+    (q : qualifier) : qualifier :=
+  match q with
+  | tqual D P =>
+      tqual (set_map f D)
+        (fun s' =>
+           exists s : LStoreOnT D,
+             lstore_on_rekey f Hf s = s' /\ P s)
+  end.
+
+Definition qual_shift_from (k : nat) (q : qualifier) : qualifier :=
+  qual_rename (logic_var_shift_from k) (logic_var_shift_from_inj k) q.
+
+#[global] Instance shift_qual_inst : Shift qualifier :=
+  qual_shift_from.
+Arguments shift_qual_inst /.
+
+Lemma qual_shift_from_vars k q :
+  qual_vars (qual_shift_from k q) = lvars_shift_from k (qual_vars q).
+Proof.
+  destruct q. reflexivity.
+Qed.
+
+Lemma qual_open_shift_from_under_gen j k x q :
+  j <= k ->
+  qual_open_atom (S k) x (qual_shift_from j q) =
+  qual_shift_from j (qual_open_atom k x q).
+Proof.
+  intros Hjk.
+  destruct q as [D P].
+  apply qual_ext; cbn [qual_lvars qual_prop qual_open_atom qual_shift_from
+    qual_rename].
+  - apply lvars_open_shift_from_under_gen. exact Hjk.
+  - intros s1 s2 Hs.
+    split.
+    + intros [s [Hshift HP]].
+      exists (lstore_on_open_front k x s). split.
+      * apply lstore_on_ext.
+        rewrite <- Hs.
+        change (lso_store (lstore_on_shift_from j (lstore_on_open_front k x s)) =
+          lso_store s1).
+        rewrite lstore_on_shift_from_open_front by exact Hjk.
+        replace (lstore_on_shift_from j s) with
+          (lstore_on_open_back (S k) x
+            (set_map (logic_var_shift_from j) D) s1)
+          by (symmetry; exact Hshift).
+        rewrite lstore_on_open_front_back. reflexivity.
+      * rewrite lstore_on_open_back_front. exact HP.
+    + intros [s [Hshift HP]].
+      exists (lstore_on_open_back k x D s). split.
+      * apply lstore_on_ext.
+        change (lso_store (lstore_on_shift_from j (lstore_on_open_back k x D s)) =
+          lso_store (lstore_on_open_back (S k) x
+            (set_map (logic_var_shift_from j) D) s1)).
+        rewrite lstore_on_shift_from_open_back by exact Hjk.
+        replace (lso_store (lstore_on_shift_from j s)) with (lso_store s2)
+          by (rewrite <- Hshift; reflexivity).
+        transitivity (lstore_swap (LVBound (S k)) (LVFree x) (lso_store s1)).
+        -- rewrite Hs. reflexivity.
+        -- unfold lstore_on_open_back. cbn [lso_store]. reflexivity.
+      * exact HP.
+Qed.
+
+Lemma qual_open_shift_from_lc_fresh k x q :
+  lvars_lc_at k (qual_vars q) ->
+  x ∉ qual_dom q ->
+  qual_open_atom k x (qual_shift_from k q) = q.
+Proof.
+  intros Hlc Hx.
+  destruct q as [D P].
+  apply qual_ext; cbn [qual_vars qual_dom qual_lvars qual_prop
+    qual_open_atom qual_shift_from qual_rename].
+  - apply lvars_open_shift_from_lc_at_fresh; assumption.
+  - intros s1 s2 Hs.
+    assert (Hshift_id : forall (s : LStoreOnT D),
+      lso_store (lstore_on_shift_from k s) = lso_store s).
+    {
+      intros s.
+      apply lstore_shift_from_below_id. exact Hlc.
+    }
+    assert (Hopen_id :
+      lso_store
+        (lstore_on_open_back k x (lvars_shift_from k D) s1) =
+      lso_store s1).
+    {
+      apply storeA_swap_fresh.
+      - intros Hbad.
+        pose proof Hbad as HbadD.
+        pose proof (lso_dom s1) as Hdoms1.
+        change (LVBound k ∈ dom (lso_store s1 : LStoreT)) in HbadD.
+        rewrite Hdoms1 in HbadD.
+        apply elem_of_set_swap in HbadD.
+        unfold swap in HbadD.
+        rewrite decide_True in HbadD by reflexivity.
+        destruct (decide (LVFree x = LVBound k)) as [Hbad_eq|_];
+          [discriminate|].
+        apply elem_of_map in HbadD as [v [Hv HvD]].
+        destruct v as [n|a]; cbn [logic_var_shift_from] in Hv.
+        + repeat case_decide; inversion Hv.
+        + inversion Hv. subst a.
+          apply Hx. apply lvars_fv_elem. exact HvD.
+      - intros Hbad.
+        pose proof Hbad as HbadD.
+        pose proof (lso_dom s1) as Hdoms1.
+        change (LVFree x ∈ dom (lso_store s1 : LStoreT)) in HbadD.
+        rewrite Hdoms1 in HbadD.
+        apply elem_of_set_swap in HbadD.
+        unfold swap in HbadD.
+        destruct (decide (LVBound k = LVFree x)) as [Hbad_eq|Hneq];
+          [discriminate|].
+        rewrite decide_False in HbadD by (intros Heq; apply Hneq; symmetry; exact Heq).
+        rewrite decide_True in HbadD by reflexivity.
+        apply elem_of_map in HbadD as [v [Hv HvD]].
+        destruct v as [n|a]; cbn [logic_var_shift_from] in Hv.
+        + destruct (decide (k <= n)) as [Hkn|Hkn].
+          * inversion Hv. lia.
+          * inversion Hv. subst n.
+            specialize (Hlc k ltac:(apply lvars_bv_elem; exact HvD)).
+            lia.
+        + discriminate.
+    }
+    split.
+    + intros [s [Hshift HP]].
+      pose proof (f_equal (@lso_store V _) Hshift) as Hshift_store.
+      assert (Hs_eq : s = s2).
+      {
+        apply lstore_on_ext.
+        transitivity (lso_store (lstore_on_shift_from k s)).
+        - symmetry. apply Hshift_id.
+        - transitivity
+            (lso_store (lstore_on_open_back k x (lvars_shift_from k D) s1)).
+          + exact Hshift_store.
+          + rewrite Hopen_id. exact Hs.
+      }
+      subst s. exact HP.
+    + intros HP.
+      exists s2. split; [|exact HP].
+      apply lstore_on_ext.
+      transitivity (lso_store s2).
+      { apply Hshift_id. }
+      transitivity (lso_store s1).
+      { symmetry. exact Hs. }
+      symmetry. exact Hopen_id.
+Qed.
+
+Lemma qual_open_atom_fresh_lc_at k x q :
+  (forall n, n ∈ lvars_bv (qual_vars q) -> n < k) ->
+  x ∉ qual_dom q ->
+  qual_open_atom k x q = q.
+Proof.
+  intros Hbelow Hx.
+  destruct q as [D P].
+  apply qual_ext; cbn [qual_vars qual_dom qual_lvars qual_prop
+    qual_open_atom].
+  - apply lvars_open_fresh_index.
+    + intros Hk. specialize (Hbelow k Hk). lia.
+    + exact Hx.
+  - intros s1 s2 Hs.
+    assert (Hopen_id :
+      lso_store (lstore_on_open_back k x D s1) = lso_store s1).
+    {
+      apply storeA_swap_fresh.
+      - intros Hbad.
+        pose proof Hbad as HbadD.
+        change (LVBound k ∈ dom (lso_store s1 : LStoreT)) in HbadD.
+        rewrite (lso_dom s1) in HbadD.
+        apply elem_of_set_swap in HbadD.
+        unfold swap in HbadD.
+        rewrite decide_True in HbadD by reflexivity.
+        destruct (decide (LVFree x = LVBound k)) as [Hbad_eq|_];
+          [discriminate|].
+        apply Hx. apply lvars_fv_elem. exact HbadD.
+      - intros Hbad.
+        pose proof Hbad as HbadD.
+        change (LVFree x ∈ dom (lso_store s1 : LStoreT)) in HbadD.
+        rewrite (lso_dom s1) in HbadD.
+        apply elem_of_set_swap in HbadD.
+        unfold swap in HbadD.
+        destruct (decide (LVBound k = LVFree x)) as [Hbad_eq|Hneq];
+          [discriminate|].
+        rewrite decide_False in HbadD by
+          (intros Heq; apply Hneq; symmetry; exact Heq).
+        rewrite decide_True in HbadD by reflexivity.
+        specialize (Hbelow k ltac:(apply lvars_bv_elem; exact HbadD)).
+        lia.
+    }
+    assert (Hback_eq : lstore_on_open_back k x D s1 = s2).
+    {
+      apply lstore_on_ext.
+      rewrite Hopen_id. exact Hs.
+    }
+    split.
+    + intros HP.
+      rewrite Hback_eq in HP. exact HP.
+    + intros HP.
+      rewrite Hback_eq. exact HP.
+Qed.
+
+End Qualifier.
+
+Notation type_qualifier := (qualifier (V := value)) (only parsing).
